coq_fsub/coq_fsub_all/DecidabilityWF.v
@@ -1,11 +1,15 @@
 Set Implicit Arguments.
 Require Import Metalib.Metatheory.
 Require Import Program.Equality.
-Require Export Progress.
+Require Export Antisymmetry.
 Require Export Coq.micromega.Lia.
 
-(* The first one is for recursive,
-the second one is for universal. *)
+(* Use the old measure to prove deciability of well-formedness
+
+the measure for subtyping will be fixed up in Decidability.v
+*)
+Module WF_dec_aux.
+
 Definition menv := list (nat * nat).
 Notation empty_menv := (@nil (nat * nat)).
 
@@ -28,6 +32,7 @@ Fixpoint findX  (x:var) (G: list (atom * nat)) :=
 Fixpoint bindings_rec (G:genv) (E: menv) (n: nat) (T:typ) : nat :=
   match T with
   | typ_nat => 1
+  | typ_top => 1
   | typ_bot => 1
   | typ_fvar x => 1 + match findX x G with
                       | Some k => k
@@ -42,12 +47,15 @@ Fixpoint bindings_rec (G:genv) (E: menv) (n: nat) (T:typ) : nat :=
   | typ_all A B =>
     let i := bindings_rec G E n A in
     S (i + (bindings_rec G ((S n, i) :: E) (S n) B))
+  | typ_all_lb A B =>
+    let i := bindings_rec G E n A in
+    S (i + (bindings_rec G ((S n, i) :: E) (S n) B))
   | typ_mu A => 
        let i := bindings_rec G ((S n , 1) :: E) (S n) A in
        S (bindings_rec G ((S n, i) :: E) (S n) A)
-  | typ_rcd_nil => 1
+  (* | typ_rcd_nil => 1
   | typ_rcd_cons i T1 T2 =>
-      S (bindings_rec G E n T1) + (bindings_rec G E n T2)
+      S (bindings_rec G E n T1) + (bindings_rec G E n T2) *)
   end.
 
 Fixpoint mk_benv (E:env) : genv :=
@@ -55,6 +63,9 @@ Fixpoint mk_benv (E:env) : genv :=
   | nil => nil
   | (_, bind_typ _)::E' => mk_benv E'
   | (X, bind_sub U)::E' => 
+        let G := mk_benv E' in 
+        (X, bindings_rec G nil 0 U) :: G
+  | (X, bind_sub_lb U)::E' => 
         let G := mk_benv E' in 
         (X, bindings_rec G nil 0 U) :: G
   end.
@@ -91,6 +102,8 @@ Qed.
 Inductive WFC :  typ -> nat -> Prop :=
 | WC_nat: forall k,
     WFC typ_nat k
+| WC_top: forall k,
+    WFC typ_top k
 | WC_bot: forall k,
     WFC typ_bot k
 | WC_fvar: forall X k,
@@ -106,24 +119,30 @@ Inductive WFC :  typ -> nat -> Prop :=
     WFC A n ->
     WFC B (S n) ->
     WFC (typ_all A B) n
+| WC_all_lb : forall A B n,
+    WFC A n ->
+    WFC B (S n) ->
+    WFC (typ_all_lb A B) n
 | WC_rec: forall A n,
     WFC A (S n) ->
     WFC (typ_mu A) n
 | WC_label: forall l A k,
     WFC A k ->
     WFC (typ_label l A) k
-| WC_nil: forall k,
+(* | WC_nil: forall k,
     WFC typ_rcd_nil k
 | WC_cons: forall i A B k,
     WFC A k ->
     WFC B k ->
-    WFC (typ_rcd_cons i A B) k
+    WFC (typ_rcd_cons i A B) k *)
 .
 
 (* WFC typ n : type with < k binded variables *)
 Inductive WFD :  typ -> nat -> Prop :=
 | WD_nat: forall k,
     WFD typ_nat k
+| WD_top: forall k,
+    WFD typ_top k
 | WD_bot: forall k,
     WFD typ_bot k
 | WD_fvar: forall X k,
@@ -142,15 +161,19 @@ Inductive WFD :  typ -> nat -> Prop :=
     WFD A n ->
     WFD B (S n) ->
     WFD (typ_all A B) n
+| WD_all_lb: forall A B n,
+    WFD A n ->
+    WFD B (S n) ->
+    WFD (typ_all_lb A B) n
 | WD_rcd: forall l A k,
     WFD A k ->
     WFD (typ_label l A) k
-| WD_nil: forall k,
+(* | WD_nil: forall k,
     WFD typ_rcd_nil k
 | WD_cons: forall i A B k,
     WFD A k ->
     WFD B k ->
-    WFD (typ_rcd_cons i A B) k
+    WFD (typ_rcd_cons i A B) k *)
 .
 
 Inductive WFE : menv -> nat -> Prop :=
@@ -308,6 +331,12 @@ Proof with auto.
     replace ((S (S n), bindings_rec G E n A) :: addone E)
     with (addone ((S n, bindings_rec G E n A) :: E))...
   -
+    (* all lb *)
+    simpl. f_equal.
+    rewrite <- IHWFC1.
+    replace ((S (S n), bindings_rec G E n A) :: addone E)
+    with (addone ((S n, bindings_rec G E n A) :: E))...
+  -
     simpl...
     f_equal...
     assert (bindings_rec G ((S (S n), 1) :: addone E) (S (S n)) A =
@@ -323,16 +352,19 @@ Qed.
 Fixpoint close_tt_rec (K : nat) (Z : atom) (T : typ) {struct T} : typ :=
   match T with
   | typ_nat         => typ_nat      
-  | typ_bot         => typ_bot              
+  | typ_top         => typ_top     
+  | typ_bot         => typ_bot         
   | typ_bvar J      => typ_bvar J
   | typ_fvar X      => if X == Z then typ_bvar K else typ_fvar X 
   | typ_arrow T1 T2 => typ_arrow (close_tt_rec K Z T1) (close_tt_rec K Z T2)
   | typ_mu T        => typ_mu (close_tt_rec (S K) Z T)
   | typ_all A B     => typ_all (close_tt_rec K Z A) 
                                 (close_tt_rec (S K) Z B)
+  | typ_all_lb A B  => typ_all_lb (close_tt_rec K Z A) 
+                                   (close_tt_rec (S K) Z B)
   | typ_label l T => typ_label l (close_tt_rec K Z T)
-  | typ_rcd_nil => typ_rcd_nil
-  | typ_rcd_cons i A B => typ_rcd_cons i (close_tt_rec K Z A) (close_tt_rec K Z B)
+  (* | typ_rcd_nil => typ_rcd_nil
+  | typ_rcd_cons i A B => typ_rcd_cons i (close_tt_rec K Z A) (close_tt_rec K Z B) *)
   end.
 
 Definition close_tt T X := close_tt_rec 0 X T.
@@ -411,6 +443,13 @@ Proof with auto.
     specialize_x_and_L X L.
     apply close_wfc with (X:=X) in H1.
     rewrite <- close_open_reverse in H1...
+  - (* WFC_all_lb *)
+    constructor...
+    apply WFC_add_one.
+    pick_fresh X.
+    specialize_x_and_L X L.
+    apply close_wfc with (X:=X) in H1.
+    rewrite <- close_open_reverse in H1...
 Qed.
 
 Lemma close_type_wfd: forall A,
@@ -424,6 +463,12 @@ Proof with auto.
     apply close_wfd with (X:=X) in H0.
     rewrite <-close_open_reverse in H0...
   - (* WFD_all *)
+    constructor...
+    pick_fresh X.
+    specialize_x_and_L X L.
+    apply close_wfd with (X:=X) in H1.
+    rewrite <- close_open_reverse in H1...
+  - (* WFD_all_lb *)
     constructor...
     pick_fresh X.
     specialize_x_and_L X L.
@@ -518,6 +563,14 @@ Proof with auto using WFE_S_n.
     lia.
     lia.
   - (* typ_all *)
+    simpl...
+    f_equal.
+    rewrite <- IHWFD1... f_equal.
+    replace (S (n0 - q)) with (S n0 - q) by lia.
+    assert  ( ((S n0 - q, bindings_rec G E n0 A) :: minusk E q) = minusk ((S n0, bindings_rec G E n0 A)::E) q) as W2 by (simpl;auto).
+    rewrite W2.
+    rewrite <- IHWFD2... lia.
+  - (* typ_all_lb *)
     simpl...
     f_equal.
     rewrite <- IHWFD1... f_equal.
@@ -621,6 +674,14 @@ Proof with eauto.
     rewrite IHWFD2...
     intros.
     apply minus_in_for_bindings...
+  -
+    simpl. f_equal.
+    rewrite IHWFD1... f_equal.
+    remember (bindings_rec G E1 n A).
+    rewrite_env (((S n, n0) :: E1) ++ E2).
+    rewrite IHWFD2...
+    intros.
+    apply minus_in_for_bindings...
 Qed.
 
 
@@ -682,16 +743,35 @@ Proof with auto.
   intros. generalize dependent E.
   induction H;try solve [simpl in H0;simpl;intros;auto];intros...
   - simpl. destruct T...
-    simpl. destruct (X0==X)...
-    subst. exfalso.
-    apply H0. simpl...
+    + simpl. destruct (X0==X)...
+      subst. exfalso.
+      apply H0. simpl...
+    + simpl. destruct (X0==X)...
+      subst. exfalso.
+      apply H0. simpl...
   - simpl. f_equal. destruct T...
-    rewrite IHWFD... 2:{ constructor... apply WFE_find_none... }
-    simpl. f_equal. f_equal. f_equal.
-    rewrite IHWFD... { constructor... apply WFE_find_none... }
-  - simpl. f_equal. destruct T... simpl in H0.
-    rewrite IHWFD1... f_equal.
-    rewrite IHWFD2... { constructor... apply WFE_find_none... }
+    +
+      rewrite IHWFD... 2:{ constructor... apply WFE_find_none... }
+      simpl. f_equal. f_equal. f_equal.
+      rewrite IHWFD... { constructor... apply WFE_find_none... }
+    +
+      rewrite IHWFD... 2:{ constructor... apply WFE_find_none... }
+      simpl. f_equal. f_equal. f_equal.
+      rewrite IHWFD... { constructor... apply WFE_find_none... }
+  - simpl. f_equal. destruct T...
+    + simpl in H0.
+      rewrite IHWFD1... f_equal.
+      rewrite IHWFD2... { constructor... apply WFE_find_none... }
+    + simpl in H0.
+      rewrite IHWFD1... f_equal.
+      rewrite IHWFD2... { constructor... apply WFE_find_none... }
+  - simpl. f_equal. destruct T...
+    + simpl in H0.
+      rewrite IHWFD1... f_equal.
+      rewrite IHWFD2... { constructor... apply WFE_find_none... }
+    + simpl in H0.
+      rewrite IHWFD1... f_equal.
+      rewrite IHWFD2... { constructor... apply WFE_find_none... }
 Qed.   
 
 
@@ -731,13 +811,80 @@ Proof with auto.
         { rewrite IHE with (Q:= Q)... 2:{ inversion H... }
           rewrite_alist (mk_benv (a ~ bind_sub t ++ E)). f_equal.
           apply findX_extend_spec...
-          { inversion H;subst. apply in_split in H0. destruct H0 as [? [? ?]].
-            rewrite H0 in H4. apply WF_from_binds_typ_strong in H4.
-            apply WF_type in H4... }
+          { inversion H;subst. apply WF_from_binds_typ in H0...
+            apply WF_type in H0... }
           { rewrite_env (nil ++ a ~ bind_sub t ++ E) in H.
             apply notin_from_wf_env in H.
             assert (binds X (bind_sub Q) E)...
             apply notin_fv_tt_fv_env with (E:=E) (Y:=X)...
+          }
+        }
+      * simpl. destruct (X == a)...
+        { subst. inversion H;subst.
+          exfalso. apply H6.
+          apply in_split in H0. destruct H0 as [E1 [E2 H1]].
+          rewrite H1. rewrite dom_app. simpl... }
+        { rewrite IHE with (Q:= Q)... 2:{ inversion H... }
+          rewrite_alist (mk_benv (a ~ bind_sub t ++ E)). f_equal.
+          apply findX_extend_spec...
+          { inversion H;subst. apply WF_from_binds_typ in H0...
+            apply WF_type in H0... }
+          { rewrite_env (nil ++ a ~ bind_sub_lb t ++ E) in H.
+            apply notin_from_wf_env_lb in H.
+            assert (binds X (bind_sub Q) E)...
+            apply notin_fv_tt_fv_env with (E:=E) (Y:=X)...
+          }
+        }
+      * inversion H...
+Qed.
+
+
+Lemma findX_sem_lb: forall E X Q,
+  wf_env E ->
+  binds X (bind_sub_lb Q) E ->
+  findX X (mk_benv E) = Some (bindings_rec (mk_benv E) nil 0 Q).
+Proof with auto.
+  induction E.
+  - intros. inversion H0.
+  - intros. destruct H0.
+    + destruct a. inversion H0;subst.
+      simpl. rewrite eq_dec_refl.
+      f_equal. rewrite_alist (mk_benv (X ~ bind_sub Q ++ E)).
+      apply findX_extend_spec...
+      { inversion H;subst. apply WF_type in H5... }
+      rewrite_env (nil ++ X ~ bind_sub_lb Q ++ E) in H.
+      apply notin_from_wf_env_lb in H...
+    + destruct a. simpl. destruct b...
+      * simpl. destruct (X == a)...
+        { subst. inversion H;subst.
+          exfalso. apply H6.
+          apply in_split in H0. destruct H0 as [E1 [E2 H1]].
+          rewrite H1. rewrite dom_app. simpl... }
+        { rewrite IHE with (Q:= Q)... 2:{ inversion H... }
+          rewrite_alist (mk_benv (a ~ bind_sub t ++ E)). f_equal.
+          apply findX_extend_spec...
+          { inversion H;subst. apply WF_from_binds_typ_lb in H0...
+            apply WF_type in H0... }
+          { rewrite_env (nil ++ a ~ bind_sub t ++ E) in H.
+            apply notin_from_wf_env in H.
+            assert (binds X (bind_sub_lb Q) E)...
+            apply notin_fv_tt_fv_env_lb with (E:=E) (Y:=X)...
+          }
+        }
+      * simpl. destruct (X == a)...
+        { subst. inversion H;subst.
+          exfalso. apply H6.
+          apply in_split in H0. destruct H0 as [E1 [E2 H1]].
+          rewrite H1. rewrite dom_app. simpl... }
+        { rewrite IHE with (Q:= Q)... 2:{ inversion H... }
+          rewrite_alist (mk_benv (a ~ bind_sub t ++ E)). f_equal.
+          apply findX_extend_spec...
+          { inversion H;subst. apply WF_from_binds_typ_lb in H0...
+            apply WF_type in H0... }
+          { rewrite_env (nil ++ a ~ bind_sub_lb t ++ E) in H.
+            apply notin_from_wf_env_lb in H.
+            assert (binds X (bind_sub_lb Q) E)...
+            apply notin_fv_tt_fv_env_lb with (E:=E) (Y:=X)...
           }
         }
       * inversion H...
@@ -787,6 +934,23 @@ Proof with auto.
       rewrite H1.
       erewrite <- bindings_find_notin... 
   - (* all *)
+    dependent destruction H1.
+    simpl. f_equal.
+    rewrite IHA1... f_equal.
+    remember ((S n,
+    bindings_rec G (E1 ++ (0, bindings_rec G (E1 ++ E2) n B - 1) :: E2) n A1)) as R1.
+    assert (bindings_rec G (E1++E2) n B = bindings_rec G (R1 :: E1++E2) (S n) B) as Q1.
+    subst.
+    apply bindings_close...
+    rewrite Q1.    
+    rewrite_alist ((R1 :: E1) ++ (0, bindings_rec G ((R1 :: E1) ++ E2) (S n) B - 1) :: E2).
+    rewrite <- IHA2...
+    rewrite_alist (R1 :: E1 ++E2)...
+    subst...
+    rewrite_env (R1 :: E1 ++ E2).
+    subst.
+    apply WFE_S_n...
+  - (* all_lb *)
     dependent destruction H1.
     simpl. f_equal.
     rewrite IHA1... f_equal.
@@ -947,6 +1111,24 @@ Proof with auto.
     rewrite_alist ((S n, K) :: (E1 ++ E2)).
     rewrite <- bindings_close with (B:=B)...
 
+  - (* lb *)
+    simpl.
+    dependent destruction H. simpl in H1.
+    simpl in IHA1. rewrite IHA1... f_equal. f_equal.
+
+    remember (bindings_rec (mk_benv G) (E1 ++ (0, bindings_rec (mk_benv G) (E1 ++ E2) n B) :: E2) n A1) as K.
+
+    rewrite_env (
+      ((S n, K)
+      :: E1) ++ E2
+    ).
+    simpl in IHA2. rewrite IHA2 at 1...
+
+    2:{ constructor... apply WFE_find_none... }
+
+    rewrite_alist ((S n, K) :: (E1 ++ E2)).
+    rewrite <- bindings_close with (B:=B)...
+
   -
     simpl.
     dependent destruction H. simpl in H0.
@@ -983,10 +1165,10 @@ Proof with auto.
     
   - simpl. f_equal. simpl in IHA. simpl in H0.
     rewrite IHA... inversion H...
-  -
+  (* -
     inversion H;subst. simpl in H0.
     simpl. f_equal. simpl in IHA1. simpl in IHA2.
-    rewrite IHA1... 
+    rewrite IHA1...  *)
 Qed.
 
 
@@ -1077,6 +1259,14 @@ Proof with auto.
     specialize (IHA2 (S n) _ _ H0).
     lia.
   - simpl.
+    specialize (IHA1 n _ _ H).
+    assert (sub_menv
+      ((S n, (bindings_rec G R1 n A1)) :: R1)
+      ((S n, (bindings_rec G R2 n A1)) :: R2)).
+    { constructor... }
+    specialize (IHA2 (S n) _ _ H0).
+    lia.
+  - simpl.
     assert (sub_menv ((S n, 1) :: R1) ((S n, 1) :: R2))...
     pose proof IHA (S n) _ _ H0.
     assert (sub_menv
@@ -1085,12 +1275,14 @@ Proof with auto.
     )...
     pose proof IHA (S n) _ _ H2. lia.
   - simpl. specialize (IHA n _ _ H). lia.
-  - simpl. specialize (IHA1 n _ _ H). specialize (IHA2 n _ _ H).
-    lia.
+  (* - simpl. specialize (IHA1 n _ _ H). specialize (IHA2 n _ _ H).
+    lia. *)
 Qed.
 
 
-Ltac solve_right_dec := right;intro v;inversion v;try inv_rt;auto.
+Ltac solve_right_dec := right;intro v;inversion v;
+(* try inv_rt; *)
+auto.
 
 
 Lemma WFC_dec : forall m A,
@@ -1104,10 +1296,12 @@ Proof with auto.
     destruct (IHA2 m); try solve [solve_right_dec]...
   - destruct (IHA1 m); try solve [solve_right_dec].
     destruct (IHA2 (S m)); try solve [solve_right_dec]...
+  - destruct (IHA1 m); try solve [solve_right_dec].
+    destruct (IHA2 (S m)); try solve [solve_right_dec]...
   - destruct (IHA (S m)); try solve [solve_right_dec]...
   - destruct (IHA m); try solve [solve_right_dec]...
-  - destruct (IHA1 m); try solve [solve_right_dec].
-    destruct (IHA2 (m)); try solve [solve_right_dec]...
+  (* - destruct (IHA1 m); try solve [solve_right_dec].
+    destruct (IHA2 (m)); try solve [solve_right_dec]... *)
 Qed.
 
 Lemma wf_fvar_dec: forall E (a:atom), 
@@ -1119,13 +1313,17 @@ Proof with auto.
   destruct H0.
   { destruct s. destruct x.
     * left. apply WF_var with (U:=t)...
+    * left. apply WF_var_lb with (U:=t)...
     * right. intros C. inversion C;subst.
-      pose proof binds_unique _ _ _ _ _ b H2 H.
-      inversion H0.
+      { pose proof binds_unique _ _ _ _ _ b H2 H.
+        inversion H0. }
+      { pose proof binds_unique _ _ _ _ _ b H2 H.
+        inversion H0. }
   }
   { right. intros C.
     inversion C;subst.
     apply n with (Q:=bind_sub U)...
+    apply n with (Q:=bind_sub_lb U)...
   }
 Qed.
 
@@ -1143,7 +1341,7 @@ Proof with auto.
   destruct H...
 Qed.  
 
-Lemma rt_type_dec: forall A,
+(* Lemma rt_type_dec: forall A,
   { rt_type A } + { ~ rt_type A }.
 Proof with auto.
   intros. destruct A;try solve [left;constructor|right;intros C;inversion C].
@@ -1156,7 +1354,7 @@ Proof with auto.
   - simpl. destruct IHA2.
     + left. apply union_iff. right...
     + destruct (i == a)...
-Qed.
+Qed. *)
 
 
 Lemma wf_dec_aux : forall G k A E,
@@ -1226,6 +1424,46 @@ Proof with auto.
         specialize_x_and_L Y L.
         apply WF_replacing_var with (X:=Y)...
 
+
+    + (* all lb *)
+      simpl in H0.
+      destruct IHA1 with (E:=E);try solve [lia|solve_right_dec]...
+      assert (type A1). { apply WF_type with (E:=E)... }
+      destruct (WFC_dec 0 A2).
+      2:{ right. intros C. apply WF_type in C.
+          inversion C;subst. apply n.
+          pick_fresh X.
+          apply type_open_tt_WFC with (X:=X)... }
+
+      pick fresh X.
+      remember (open_tt A2 X) as Q1.
+      destruct IHk with (A:=Q1) (E:= X ~ bind_sub_lb A1 ++ E)...
+      { subst. rewrite_alist (empty_menv ++ empty_menv).
+        rewrite bindings_find...
+        rewrite bindings_add... unfold zero. simpl.
+        simpl.
+        
+        eapply le_trans.
+        { apply sub_menv_sem with 
+            (R2:=((1, bindings_rec G empty_menv 0 A1) :: empty_menv)). 
+          constructor...
+          rewrite findX_notin...
+          simpl.
+          apply bindings_rec_ge_1. }
+        lia.
+      }
+      * (* A2 is well formed *)
+        left. apply WF_all_lb with (L:={{X}} \u fv_tt A2 \u dom E)...
+        intros. subst Q1.
+        apply WF_replacing_var_lb with (X:=X)...
+
+      * (* A2 is not well formed *)
+        right. intros C. apply n. subst Q1.
+        dependent destruction C. pick_fresh Y.
+        specialize_x_and_L Y L.
+        apply WF_replacing_var_lb with (X:=Y)...
+
+
     + (* mu *)
       simpl in H0.
 
@@ -1238,7 +1476,7 @@ Proof with auto.
       pick fresh X.
       remember (open_tt A X) as Q1.
       remember (open_tt A (typ_label X (open_tt A X))) as Q2.
-      destruct IHk with (A:=Q1) (E:= X ~ bind_sub typ_bot ++ E)...
+      destruct IHk with (A:=Q1) (E:= X ~ bind_sub typ_top ++ E)...
       { subst. rewrite_alist (empty_menv ++ empty_menv).
         rewrite bindings_find...
         rewrite bindings_add... unfold zero. simpl.
@@ -1252,7 +1490,7 @@ Proof with auto.
         lia. }
       
       * (* open_tt A X is well-formed  *)
-        destruct IHk with (A:=Q2) (E:= X ~ bind_sub typ_bot ++ E)...
+        destruct IHk with (A:=Q2) (E:= X ~ bind_sub typ_top ++ E)...
         { subst. rewrite_alist (empty_menv ++ empty_menv).
           rewrite bindings_find...
           2:{ apply WF_type in w0... }
@@ -1284,12 +1522,12 @@ Proof with auto.
            rewrite eq_dec_refl in w1.
            rewrite <- subst_tt_fresh in w1...
            (* stuck: how to get 
-           WF (X0 ~ bind_sub typ_bot ++ E) 
+           WF (X0 ~ bind_sub typ_top ++ E) 
               (open_tt A (typ_label X0 (open_tt A X0)))
 
            from 
 
-           WF ((X0, bind_sub typ_bot) :: E)
+           WF ((X0, bind_sub typ_top) :: E)
              (open_tt A (typ_label X (open_tt A X0)))           
             *)
            apply WF_renaming_tl with (X:=X) (Y:=X0) in w1...
@@ -1314,827 +1552,22 @@ Proof with auto.
     simpl in H0.
     destruct IHA with (E:=E);try solve [lia|solve_right_dec]...
 
-  + (* rcd *)
+  (* + rcd
     simpl in H0.
     destruct IHA1 with (E:=E);try solve [lia|solve_right_dec]...
     destruct IHA2 with (E:=E);try solve [lia|solve_right_dec]...
     destruct (rt_type_dec A2);try solve [lia|solve_right_dec]...
-    destruct (collectLabelDec a A2);try solve [lia|solve_right_dec]...
+    destruct (collectLabelDec a A2);try solve [lia|solve_right_dec]... *)
 Qed.
 
+End WF_dec_aux.
 
 Lemma wf_dec : forall  A E,
   uniq E -> 
     {WF E A} + {~ WF E A}.
 Proof with auto.
   intros.
-  apply wf_dec_aux with (k:=bindings_rec nil nil 0 A) (G:=nil)...
+  apply WF_dec_aux.wf_dec_aux with (k:=WF_dec_aux.bindings_rec nil nil 0 A) (G:=nil)...
 Qed.
 
 
-
-Lemma binds_key_dom_dec: forall (E: env) X,
-  {X \in dom E} + {X \notin dom E}.
-Proof with auto.
-induction E...
-intros.
-destruct a.
-destruct (X==a)...
--
-  subst. left. simpl...
--
-  destruct IHE with (X:=X)...
-  left. simpl...
-Qed.
-
-Lemma wf_env_dec: forall E,
-    {wf_env E} + {~wf_env E}.
-Proof with auto.  
-  induction E...
-  destruct IHE.
-  -
-    pose proof wf_dec.
-    assert (Ht:=w).
-    apply uniq_from_wf_env in Ht.
-    pose proof binds_key_dom_dec.
-    destruct a.
-    destruct b.
-    +
-      destruct H with (E:=E) (A:=t)...
-      destruct H0 with (E:=E) (X:=a)...
-      *
-        right.
-        intros v.
-        dependent destruction v...
-      *
-        left.
-        constructor...
-      *
-        right.
-        intros v.
-        dependent destruction v...
-    +
-      destruct H with (E:=E) (A:=t)...
-      destruct H0 with (E:=E) (X:=a)...
-      *
-        right.
-        intros v.
-        dependent destruction v...
-      *
-        left.
-        constructor...
-      *
-        right.
-        intros v.
-        dependent destruction v...
-  -
-    right.
-    intros v.
-    dependent destruction v;
-      apply n...
-Qed.
-
-
-Ltac solve_bot_dec E := 
-  pose wf_env_dec as Q;destruct Q with (E:=E) as [Ql|Qr];try solve [
-  left;auto |
-  solve_right_dec  ].
-Ltac solve_bot_wfs_dec E A := 
-  match goal with
-  | H : wf_env E |- _ =>    
-    destruct (wf_dec A (uniq_from_wf_env H)); 
-    try solve [left;auto|right;intros v;dependent destruction v;auto]
-  | _ => idtac
-  end.
-
-Lemma find_var_one: forall Q G X E n,
-  X \notin dom G ->
-  bindings_rec ( G) E n Q = 
-  bindings_rec (X ~ 1 ++  G) E n Q.
-Proof with auto.
-  intros Q G X.
-  induction Q;intros...
-  + simpl. destruct (a == X)...
-    subst.
-    rewrite (findX_notin _ H)...
-  + simpl. rewrite IHQ1...
-  + simpl. rewrite IHQ1...
-  + simpl. rewrite IHQ...
-    f_equal. f_equal. f_equal.
-    f_equal. rewrite IHQ...
-  + simpl...
-  + simpl. rewrite IHQ1...
-Qed.
-
-Lemma mk_benv_dom: forall X G,
-  X `notin` dom G -> X `notin` dom (mk_benv G).
-Proof with auto.
-  induction G;intros...
-  + intros. destruct a. simpl. destruct b...
-Qed.
-
-Lemma bindings_drop_label: forall T E G t i,
-WF E T ->
-Tlookup i T = Some t ->
-S (bindings_rec (mk_benv E) G 0 t + bindings_rec (mk_benv E) G 0 (dropLabel i T)) =
-bindings_rec (mk_benv E) G 0 T.
-Proof with auto.
-  intros T.
-  induction T;intros;try solve [inversion H0]...
-  + simpl. simpl in H0. destruct (a == i).
-    * inversion H0. subst. inversion H;subst...
-      rewrite dropLable_notin with (E:=E)...
-    * inversion H;subst...
-      rewrite <- IHT2 with (t:=t) (i:=i)...
-      simpl. lia.
-Qed.
-
-Lemma subset_dec: forall A B, { A [<=] B} + { ~ A [<=] B}.
-Proof with auto.
-  intros. destruct (AtomSetImpl.subset A B) eqn:E'.
-  + apply subset_iff in E'...
-  + right. intros C. apply subset_iff in C...
-    rewrite C in E'. inversion E'.
-Qed.
-
-
-
-(* Lemma dropLabel_first_element': forall i T1 T2,
-    (* WF E (typ_rcd_cons i T1 T2) -> *)
-    dropLabel i (typ_rcd_cons i T1 T2) = T2.
-Proof with auto.
-  intros. simpl. rewrite eq_dec_refl.
-  dependent destruction H...
-  simpl...
-  destruct (i==i)...
-  apply dropLable_notin with (E:=E)...
-  destruct n...
-Qed. *)
-
-(* Lemma record_permutation_exists_aux:
-forall E j x a T1 T2,
-rt_type T2 -> a <> j ->
-equiv E (typ_rcd_cons j x (dropLabel j T2)) T2 ->
-equiv E (typ_rcd_cons j x (dropLabel j (typ_rcd_cons a T1 T2)))
-  (typ_rcd_cons a T1 T2).
-Proof with auto.
-  intros.
-  destruct H1 as [e1 e2].
-  split.
-  + inversion e1;subst;inv_rt.
-    simpl. destruct (a == j);try solve [exfalso;auto]...
-    apply sa_rcd;try solve [get_well_form;auto]...
-    - simpl. 
-      simpl. simpl in H4. admit.
-    - inversion H5;subst. constructor... *)
-
-Lemma equiv_trans: forall E P Q R,
-  equiv E P Q -> equiv E Q R -> equiv E P R.
-Proof.
-  intros.
-  destruct H. destruct H0.
-  split;apply sub_transitivity with (Q:=Q);auto.
-Qed.
-
-Lemma sub_rcd_proper: forall E a T1 T2 T1' T2',
-  sub E T1 T1' ->
-  sub E T2 T2' -> 
-  rt_type T2 -> rt_type T2' ->
-  a `notin` collectLabel T2 ->
-  sub E (typ_rcd_cons a T1 T2) (typ_rcd_cons a T1' T2').
-Proof with auto.
-  intros.
-  apply sa_rcd...
-  + get_well_form...
-  + simpl.
-    rewrite <- !KeySetProperties.add_union_singleton.
-    apply add_s_m...
-    inversion H0;subst;inv_rt...
-  + constructor;try solve [get_well_form;auto]...
-  + constructor;try solve [get_well_form;auto]...
-    inversion H0;subst;inv_rt...
-  + intros. simpl in H4, H5. destruct (a==i).
-    * inversion H4;subst. inversion H5;subst...
-    * inversion H0;subst;inv_rt...
-      apply H12 with (i:=i)...
-Qed.
-
-
-Lemma equiv_rcd_proper: forall E a T1 T2 T1' T2',
-  equiv E T1 T1' ->
-  equiv E T2 T2' -> 
-  rt_type T2 -> rt_type T2' ->
-  a `notin` collectLabel T2 ->
-  equiv E (typ_rcd_cons a T1 T2) (typ_rcd_cons a T1' T2').
-Proof with auto.
-  intros. destruct H as [H H'], H0 as [H0 H0'].
-  split.
-  { apply sub_rcd_proper... }
-  { apply sub_rcd_proper...
-    inversion H0;subst;inv_rt...
-  }
-Qed.
-
-
-Lemma sub_rcd_first_permute: forall E a b T1 T2 T3,
-  wf_env E -> WF E  (typ_rcd_cons a T1 (typ_rcd_cons b T2 T3)) ->
-  sub E (typ_rcd_cons a T1 (typ_rcd_cons b T2 T3)) 
-  (typ_rcd_cons b T2 (typ_rcd_cons a T1 T3)).
-Proof with auto.
-  intros.
-  { apply sa_rcd...
-    + simpl. rewrite <- !KeySetProperties.union_assoc.
-      rewrite KeySetProperties.union_sym with (s:= singleton a). reflexivity.
-    + inversion H0;subst. inversion H6;subst.
-      constructor... 2:{ simpl in H8... }
-      constructor... { simpl in H8 ... }
-    + intros. simpl in H1, H2.
-      assert (a <> b). { inversion H0;subst. simpl in H10... }
-      destruct (a==i), (b==i);try inversion H1; try inversion H2;subst...
-      * congruence.
-      * apply Reflexivity... inversion H0...
-      * apply Reflexivity... inversion H0... inversion H9...
-      * assert (t1 = t2) by congruence. subst.
-        apply Reflexivity... apply wf_rcd_lookup with (E:=E) in H1...
-        inversion H0... inversion H11...
-  }
-Qed.
-
-
-Lemma equiv_rcd_first_permute: forall E a b T1 T2 T3,
-  wf_env E -> WF E  (typ_rcd_cons a T1 (typ_rcd_cons b T2 T3)) ->
-  equiv E (typ_rcd_cons a T1 (typ_rcd_cons b T2 T3)) 
-  (typ_rcd_cons b T2 (typ_rcd_cons a T1 T3)).
-Proof with auto.
-  intros.
-  split.
-  { apply sub_rcd_first_permute... }
-  { apply sub_rcd_first_permute...
-    inversion H0;subst.
-    inversion H6;subst.
-    constructor... 2:{ simpl in H8... }
-    constructor... { simpl in H8 ... }
-  }
-Qed.
-
-
-
-Lemma record_permutation_exists:
-  forall j E T,
-  wf_env E -> 
-  j `in` collectLabel T ->
-  { A' |
-    equiv E (typ_rcd_cons j A' ((dropLabel j T))) T} + {~ WF E T}.
-Proof with auto.
-  intros.
-  induction T;try solve [apply empty_iff in H0;destruct H0].
-  - simpl in H0.
-    destruct (Atom.eq_dec j a).
-    + subst j. 
-      solve_bot_wfs_dec E (typ_rcd_cons a T1 T2).
-      left. exists T1.
-      rewrite dropLabel_first_element with (E:=E)...
-      apply equiv_reflexivity...
-    + solve_bot_wfs_dec E (typ_rcd_cons a T1 T2).
-      destruct (collectLabelDec j T2).
-      2:{ assert (j `notin` union (singleton a) (collectLabel T2))... }
-      destruct (IHT2 i);try solve [solve_right_dec].
-      left. destruct s. exists x.
-      simpl. destruct (a ==j);try solve [exfalso;auto]...
-      apply equiv_trans with 
-        (Q:= (typ_rcd_cons a T1 (typ_rcd_cons j x (dropLabel j T2)))).
-      * apply equiv_rcd_first_permute...
-        { destruct e. get_well_form.
-          inversion H5;subst.
-          inversion w;subst. constructor...
-          constructor... apply notin_drop_collect... } 
-      * apply equiv_rcd_proper...
-        { apply equiv_reflexivity...
-          { inversion w;subst... }
-        }
-        { inversion w;subst... }
-        { simpl. solve_notin. apply notin_drop_collect...
-          inversion w... }
-Qed.
-
-Lemma equiv_measure: forall A,
-  type4rec A -> forall B, type4rec B -> forall E,
-  sub E A B -> sub E B A ->
-  bindings_rec (mk_benv E) nil 0 A = bindings_rec (mk_benv E) nil 0 B.
-Proof with auto.
-  intros A HA;induction HA.
-  - intros B HB;induction HB;intros;
-    try solve [simpl; lia| inversion H;inv_rt|inversion H0;inv_rt|
-    inversion H1;inv_rt|
-      inversion H2;inv_rt|inversion H3;inv_rt|inversion H4;inv_rt].
-  - intros B HB;induction HB;intros;
-  try solve [simpl; lia| inversion H;inv_rt|inversion H0;inv_rt|
-  inversion H1;inv_rt|
-    inversion H2;inv_rt|inversion H3;inv_rt].
-  - intros B HB;induction HB;intros;
-  try solve [simpl; lia| inversion H;inv_rt|inversion H0;inv_rt|
-  inversion H1;inv_rt|
-    inversion H2;inv_rt|inversion H3;inv_rt| inversion H4;inv_rt].
-    apply suba_sub_tvar_chain in H.
-    apply suba_sub_tvar_chain in H0.
-    destruct H as [W1], H0 as [W2].
-    pose proof sub_tvar_chain_antisym H H0. subst. lia.
-  - intros. dependent destruction H0.
-    { dependent destruction H2. inv_rt. }
-    2:{ inv_rt. }
-    dependent destruction H1.
-    2:{ inv_rt. }
-    simpl. 
-    rewrite IHHA1 with (B:=B1)...
-    2:{ apply type_to_rec. apply WF_type with (E:=E). get_well_form... }
-    rewrite IHHA2 with (B:=B2)...
-    { apply type_to_rec. apply WF_type with (E:=E). get_well_form... }
-  - intros. rename T into A1.
-    dependent destruction H4.
-    { dependent destruction H6. inv_rt. }
-    2:{ inv_rt. }
-    dependent destruction H7.
-    2:{ inv_rt. }
-    dependent destruction H3.
-    pick_fresh X.
-    specialize_x_and_L X L.
-    specialize_x_and_L X L0.
-    specialize_x_and_L X L1.
-    specialize_x_and_L X L2.
-
-
-    assert (Eh1: sub (X ~ bind_sub typ_bot ++ E) (open_tt A1 X) (open_tt A2 X)).
-    { apply sub_nominal_inversion... }
-    assert (Eh2: sub (X ~ bind_sub typ_bot ++ E) (open_tt A2 X) (open_tt A1 X)).
-    { apply sub_nominal_inversion... }
-    simpl.
-
-    specialize (H2 _ H4 ((X ~ bind_sub typ_bot) ++ E) Eh1 Eh2).
-    assert (WFC A2 0).
-    { apply type_open_tt_WFC with (X:=X)... 
-        apply type4rec_to_type... }
-    assert (WFC A1 0).
-    { apply type_open_tt_WFC with (X:=X)... 
-        apply type4rec_to_type... }
-
-
-    rewrite_env (empty_menv ++ empty_menv) in H2...
-    pose proof H2 as H2'. simpl in H2'.
-    rewrite bindings_find in H2... 
-    rewrite bindings_add in H2... 
-    rewrite bindings_find in H2... 
-    rewrite bindings_add with (A:=A2) in H2... 
-    unfold zero in H2. simpl in H2. rewrite eq_dec_refl in H2.
-    replace (1-0) with 1 in H2...
-    rewrite_env (X ~ 1 ++ mk_benv E) in H2.
-    rewrite <- find_var_one with (X:=X) in H2...
-    2:{ apply mk_benv_dom... }
-    rewrite <- find_var_one with (X:=X) in H2...
-    2:{ apply mk_benv_dom... }
-    rewrite H2. f_equal...
-
-
-
-    specialize (H0 _ H3 ((X ~ bind_sub typ_bot) ++ E) H7 H10).
-
-    rewrite_env (empty_menv ++ empty_menv) in H0...
-    rewrite bindings_find in H0... 
-    rewrite bindings_add in H0... 
-    rewrite bindings_find in H0... 
-    rewrite bindings_add with (A:=A2) in H0... 
-    unfold zero in H0. simpl in H0. rewrite H2' in H0.
-    rewrite_env (X ~ 1 ++ mk_benv E) in H0.
-    rewrite <- find_var_one with (X:=X) in H0...
-    2:{ apply mk_benv_dom... }
-    rewrite <- find_var_one with (Q:=A2) (X:=X) in H0...
-    2:{ apply mk_benv_dom... }
-    rewrite <- find_var_one with (X:=X) in H0...
-    2:{ apply mk_benv_dom... }
-
-    rewrite_env (empty_menv ++ empty_menv) in H0...
-    rewrite bindings_find in H0...
-    replace (bindings_rec (mk_benv E) (empty_menv ++ empty_menv) 0 X) with 2 in H0.
-    2:{ simpl. rewrite findX_notin... apply mk_benv_dom... }
-    simpl in H0. rewrite bindings_add with (A:=A2) in H0...
-    simpl in H0. unfold zero in H0. rewrite Nat.sub_0_r in H0...
-
-constructor. apply WF_type with (E:=X ~ bind_sub typ_bot ++ E)...
-constructor. apply WF_type with (E:=X ~ bind_sub typ_bot ++ E)...
-
-
-- 
-  intros.
-  dependent destruction H2.
-  { dependent destruction H4. inv_rt. }
-  2:{ inv_rt. }
-  dependent destruction H3.
-  2:{ inv_rt. }
-  rename T2 into S1. rename S2 into T2.
-  rename T3 into S2.
-  inversion H1;subst.
-  pick_fresh X.
-  specialize_x_and_L X L.
-  specialize_x_and_L X L0.
-  specialize_x_and_L X L1.
-  specialize_x_and_L X L2.
-  specialize (IHHA _ H6 E H2_ H2_0).
-  simpl. rewrite IHHA. f_equal. f_equal.
-
-  rewrite_env (nil ++ X ~ bind_sub T1 ++ E) in H3.
-  apply sub_narrowing with (P:=T2) in H3...
-
-  specialize (H0 _ H7 (X ~ bind_sub T2 ++ E) H2 H3).
-
-  apply type4rec_to_type in H6.
-  get_well_form...
-  assert (WFC S1 0). { apply type_open_tt_WFC with (X:=X)... apply WF_type with (E:=X~bind_sub T2 ++ E)... }
-  assert (WFC S2 0). { apply type_open_tt_WFC with (X:=X)... apply WF_type with (E:=X~bind_sub T2 ++ E)... }
-  rewrite bindings_fvar_spec in H0...
-  rewrite bindings_fvar_spec with (A:=S2) in H0...
-
--
-  intros.
-  dependent destruction H0.
-  { dependent destruction H2. inv_rt. }
-  2:{ inv_rt. }
-  dependent destruction H1.
-  2:{ inv_rt. }
-  dependent destruction H.
-  simpl. f_equal. apply IHHA...
-
--
-  intros. dependent destruction H0.
-  { dependent destruction H2. inv_rt. }
-  dependent destruction H7;try inv_rt...
-  dependent destruction H8...
-  simpl in H3. collect_nil H3.
--
-  intros. inversion H1;subst.
-  { dependent destruction H2;try inv_rt. }
-  inversion H2;subst;try inv_rt...
-  dependent destruction H5...
-  { simpl in H13. collect_nil H13. }
-  simpl.
-  assert (equiv E (typ_rcd_cons i0 T0 T3)  (typ_rcd_cons i T1 T2)) by (split;auto)...
-  apply record_permutation in H5. unfold equiv in H5. destruct_hypos.
-  rewrite IHHA1 with (B:=x)...
-  2:{ apply type_to_rec. apply WF_type with (E:=E). get_well_form... }
-  rewrite IHHA2 with (B:=(dropLabel i (typ_rcd_cons i0 T0 T3)))...
-  2:{ apply type_to_rec. apply WF_type with (E:=E). apply WF_drop. get_well_form... }
-  pose proof bindings_drop_label (T:=typ_rcd_cons i0 T0 T3) (E:=E) empty_menv (t:=x) i.
-  rewrite H22...
-Qed.
-
-
-
-Lemma subtyping_dec : forall k A B E,
-bindings_rec (mk_benv E) nil 0 A + 
-bindings_rec (mk_benv E) nil 0 B <= k ->
-{sub E A B} + {~ sub E A B}.
-Proof with auto.
-induction k.
--
-induction A;intros;try solve [unfold bindings in *;exfalso;simpl in *;lia]...
--
-induction B.
-+
-  induction A;intros;try solve [ solve_right_dec | solve_bot_dec E]...
-
-+
-  induction A;intros;try solve [ solve_right_dec | solve_bot_dec E]...
-
-+
-  induction A;intros;try solve [ solve_right_dec | solve_bot_dec E]...
-  right. intros C. inversion C;subst. inversion H1. inv_rt.
-      
-+
-  intros. simpl in H.
-  destruct (wf_env_dec E).
-  2:{ right. intros C. apply sub_regular in C. destruct C... }
-  destruct (binds_key_dec E a).
-  *
-    pose proof uniq_from_wf_env w as u.
-    destruct s.
-    destruct x.
-    { assert (WF E t).
-      { apply WF_from_binds_typ with (x:=a)... }
-      apply WF_type in H0.
-      rewrite (findX_sem _ _ w b) in H. 
-      (* 2:{ apply binds_split in b.
-        destruct b as [E1 [E2 b]]. rewrite b in w.
-        apply wf_env_binds_not_fv_tt in w... } *)
-      destruct (IHk A t E).
-      { lia. }
-      (* apply le_S_n in H.
-      destruct (IHk _ _ _ H)... *)
-      { left. apply sa_trans_tvar with (U:=t)... }
-      { destruct (EqDec_eq a A).
-        { left. subst. apply sa_fvar... apply WF_var with (U:=t)... }
-        destruct (EqDec_eq typ_bot A).
-        { left. subst. apply sa_bot... apply WF_var with (U:=t)... }
-        right. intros C. inversion C;inv_rt;subst...
-        { assert (bind_sub t =  bind_sub U). 
-          { eapply binds_unique with (x:=a) (E:=E)... }
-          inversion H1;subst... }
-      }
-    }
-    { right. intros C. apply uniq_from_wf_env in w.
-      inversion C;subst;inv_rt.
-      { inversion H4;subst. pose proof binds_unique _ _ _ _ _ b H3 w.
-        inversion H0.  }
-      { inversion H1;subst. pose proof binds_unique _ _ _ _ _ b H4 w.
-        inversion H2.  }
-      { pose proof binds_unique _ _ _ _ _ b H1 w.
-        inversion H0.  }
-    }
-
-  *
-    right. intros C.
-    inversion C;inv_rt;subst...
-    { inversion H4;subst. apply n in H3... }
-    { inversion H1;subst. apply n in H4... }
-    { apply n in H1... }
-
-
-+ intros. simpl in H.
-  induction A;intros;try solve [ solve_right_dec | solve_bot_dec E]...
-  * solve_bot_dec E. solve_bot_wfs_dec E (typ_arrow B1 B2).
-  
-  *
-    simpl in H.
-    destruct IHk with (A:=B1) (B:=A1) (E:=E); try solve [lia];
-    destruct IHk with (A:=A2) (B:=B2) (E:=E);try solve [lia];
-    try solve [solve_right_dec].
-    left. apply sa_arrow...
-
-+
-  intros. simpl in H.
-  induction A;intros;try solve [ solve_right_dec]...
-  * solve_bot_dec E. solve_bot_wfs_dec E (typ_all B1 B2).
-
-  *
-    destruct (IHk A1 B1 E); try solve [solve_right_dec].
-    { simpl in H. lia. }
-    destruct (IHk B1 A1 E); try solve [solve_right_dec].
-    { simpl in H. lia. }
-
-
-    (* destruct (EqDec_eq A1 B1);try solve [solve_right_dec]. *)
-    (* rename A1 into A. *)
-    (* rename A2 into B1. *)
-
-    destruct (wf_env_dec E).
-    2:{ right. intros C. apply sub_regular in C. destruct C as [? [? ?]]... }
-    pose proof uniq_from_wf_env w as u.
-    (* destruct (wf_dec A1 u);try solve [solve_right_dec]. *)
-
-    pick_fresh X1.
-    assert (uniq ((X1 ~ bind_sub A1) ++ E)) as u2...
-    assert (uniq ((X1 ~ bind_sub B1) ++ E)) as u3...
-    destruct (wf_dec (open_tt A2 X1) u2).
-    2:{ right. intros C.
-        apply sub_regular in C. destruct C as [? [? ?]].
-        inversion H1;subst.
-        pick_fresh X2. specialize_x_and_L X2 L.
-        apply n. apply WF_replacing_var with (X:=X2)... }
-    destruct (wf_dec (open_tt B2 X1) u3).
-    2:{ right. intros C.
-        apply sub_regular in C. destruct C as [? [? ?]].
-        inversion H2;subst.
-        pick_fresh X2. specialize_x_and_L X2 L.
-        apply n. apply WF_replacing_var with (X:=X2)... }
-    
-
-    clear IHA1 IHA2 IHB1 IHB2. simpl in H.
-
-    specialize (IHk (open_tt A2 X1) (open_tt B2 X1)
-    (X1 ~ bind_sub B1 ++ E)).
-
-    rewrite <- bindings_fvar_spec with (X:=X1)in H...
-    2:{ apply type_open_tt_WFC with (X:=X1)... apply WF_type in w0... }
-    2:{ get_well_form... }
-    2:{ get_well_form... apply WF_type in H4... }
-    
-    rewrite <- bindings_fvar_spec with (X:=X1)in H...
-    2:{ apply type_open_tt_WFC with (X:=X1)... apply WF_type in w1... }
-    2:{ get_well_form... }
-    2:{ get_well_form... apply WF_type in H5... } 
-
-    assert (Eq: bindings_rec (mk_benv E) empty_menv 0 A1 = bindings_rec (mk_benv E) empty_menv 0 B1).
-    { apply equiv_measure...
-      { apply type_to_rec. apply WF_type with (E:=E). get_well_form... }
-      { apply type_to_rec. apply WF_type with (E:=E). get_well_form... }
-    }
-    rewrite Eq in *.
-
-    destruct IHk.
-    { simpl in H. simpl. rewrite Eq in H. lia. }
-    { left.
-      apply sa_all with (L:={{X1}} \u fv_tt A1 \u fv_tt A2 \u fv_tt B1 \u fv_tt B2 \u dom E);intros...
-      (* { apply Reflexivity... } { apply Reflexivity... } *)
-      apply sub_replacing_var with (X:=X1)...
-      get_well_form...
-    }
-    { right. intros. intros C.
-      inversion C;inv_rt. subst. pick_fresh X2.
-      specialize_x_and_L X2 L.
-      apply n. apply sub_replacing_var with (X:=X2)...
-      get_well_form... }
-
-
-+ 
-  intros. simpl in H.
-  induction A;intros;try solve [ solve_right_dec]...
-  * solve_bot_dec E. solve_bot_wfs_dec E (typ_mu B).
-
-  *
-    destruct (wf_env_dec E).
-    2:{ right. intros C. apply sub_regular in C. destruct C as [? [? ?]]... }
-    pose proof uniq_from_wf_env w as u.
-
-    pick_fresh X1. assert (uniq ((X1 ~ bind_sub typ_bot) ++ E)) as u2...
-    
-    destruct (wf_dec (open_tt A X1) u2).
-    2:{ right. intros C. apply n.
-        inversion C;inv_rt. subst.
-        pick_fresh X2. specialize_x_and_L X2 L.
-        apply WF_replacing_var with (X:=X2)... }
-    destruct (wf_dec (open_tt B X1) u2).
-    2:{ right. intros C. apply n.
-        inversion C;inv_rt. subst.
-        pick_fresh X2. specialize_x_and_L X2 L.
-        apply WF_replacing_var with (X:=X2)... }
-
-    clear IHA IHB. simpl in H.
-
-    specialize (IHk (open_tt A (typ_label X1 (open_tt A X1)))
-    (open_tt B (typ_label X1 (open_tt B X1)))
-    (X1 ~ bind_sub typ_bot ++ E)).
-
-    assert (WFC A 0). { apply WF_type in w0. apply type_open_tt_WFC in w0... }
-    assert (WFC B 0). { apply WF_type in w1. apply type_open_tt_WFC in w1... }
-
-
-    rewrite bindings_find_spec' 
-      with (A:=A) (B:= typ_label X1 (open_tt A X1)) in IHk... 
-    2:{ constructor. apply WF_type in w0... }
-    rewrite bindings_find_spec' 
-      with (A:=B) (B:= typ_label X1 (open_tt B X1)) in IHk... 
-    2:{ constructor. apply WF_type in w1... }
-
-    assert (Haux: forall G E n A X, 
-      bindings_rec G E n (typ_label X A) = S (bindings_rec G E n A))...
-    rewrite !Haux in IHk. clear Haux.
-
-    rewrite bindings_fvar_spec in IHk...
-    rewrite bindings_fvar_spec in IHk...
-
-    rewrite <- findX_extend in IHk...
-    2:{ apply WFC_WFD_S... }
-    rewrite <- findX_extend in IHk...
-    2:{ apply WFC_WFD_S... }
-
-    destruct IHk.
-    { apply le_S_n in H. eapply le_trans;[|apply H].
-      apply plus_le_compat.
-      { apply sub_menv_sem. constructor...
-        simpl. lia. }
-      { apply le_S. apply sub_menv_sem.
-        constructor... simpl. lia. }
-    }
-
-    { left.
-      apply sa_rec with (L:={{X1}} \u fv_tt A \u fv_tt B \u dom E \u fl_tt A \u fl_tt B);intros...
-      { apply WF_replacing_var with (X:=X1)... }
-      { apply WF_replacing_var with (X:=X1)... }
-      {
-        apply sub_renaming_unfolding with (X:=X1)...
-      }
-    }
-    { right. intros. intros C.
-      inversion C;inv_rt. subst. pick_fresh X2.
-      specialize_x_and_L X2 L.
-      apply n. simpl.
-      apply sub_renaming_unfolding with (X:=X2)...
-    }
-
-+ 
-  intros. simpl in H.
-  induction A;intros;try solve [ solve_right_dec]...
-  * solve_bot_dec E. solve_bot_wfs_dec E (typ_label a B).
-
-  *
-    simpl in H. destruct IHk with (A:=A) (B:=B) (E:=E).
-    { lia. }
-
-    { destruct (a == a0).
-      + subst. constructor...
-      + right. intros C. inversion C;inv_rt;subst... }
-    { right. intros C. inversion C;inv_rt;subst... }
-
-+
-  intros. simpl in H.
-  induction A;intros;try solve [ solve_right_dec]...
-  * solve_bot_dec E.
-
-  * solve_bot_dec E. left. apply Reflexivity...
-
-  * solve_bot_dec E. 
-    solve_bot_wfs_dec E (typ_rcd_cons a A1 A2).
-    left. apply sa_rcd...
-    { apply KeySetProperties.subset_empty. }
-    { intros. inversion H1. }
-
-
-+
-intros. 
-induction A;intros;try solve [ solve_right_dec]...
-* solve_bot_dec E. solve_bot_wfs_dec E (typ_rcd_cons a B1 B2).
-
-* solve_bot_dec E. 
-  solve_bot_wfs_dec E (typ_rcd_cons a B1 B2).
-  right. intros C. inversion C. collect_nil H3.
-  
-*
-
-
-
-destruct (subset_dec (collectLabel (typ_rcd_cons a B1 B2)) (collectLabel (typ_rcd_cons a0 A1 A2)) );
-  try solve [ solve_right_dec].
-
-solve_bot_dec E. 
-solve_bot_wfs_dec E (typ_rcd_cons a0 A1 A2).
-solve_bot_wfs_dec E (typ_rcd_cons a B1 B2).
-
-
-destruct (@record_permutation_exists a E (typ_rcd_cons a0 A1 A2)) as [[x e]| e]...
-{ apply s... simpl. apply union_iff. left... }
-
-pose proof (e':=e).
-destruct e'.
-assert (type4rec (typ_rcd_cons a x (dropLabel a (typ_rcd_cons a0 A1 A2)))).
-{ apply type_to_rec. apply WF_type with (E:=E). get_well_form... }
-assert (type4rec (typ_rcd_cons a0 A1 A2)).
-{ apply type_to_rec. apply WF_type with (E:=E). get_well_form... }
-pose proof equiv_measure H2 H3 H0 H1.
-rewrite <- H4 in H.
-
-destruct IHk with (E:=E)
-(A:= x) (B:=B1)...
-{ simpl in H. lia... }
-2:{ right. intros C.
-    pose proof sub_transitivity H0 C.
-    inversion H5;subst.
-    specialize (H12 a x B1).
-    apply n. apply H12;simpl;rewrite eq_dec_refl...
-    }
-
-destruct IHk with (E:=E)
-(B:= B2) (A:=(dropLabel a (typ_rcd_cons a0 A1 A2)))...
-{  simpl in H. simpl. lia... }
-
--- left.
-    apply sub_transitivity with (typ_rcd_cons a x (dropLabel a (typ_rcd_cons a0 A1 A2)))...
-    apply sa_rcd...
-    { apply label_equiv in e. rewrite e... }
-    { destruct e. get_well_form... }
-    { intros.  simpl in H5. simpl in H6.
-      destruct (a == i).
-      { inversion H5. inversion H6. subst... }
-      { apply (rcd_inversion s1) with (i:=i)...
-        + get_well_form. apply rt_type_drop with (E:=E)...
-        + inversion w0... }
-    }
-
--- right.
-    intros C.
-    pose proof sub_transitivity H0 C.
-    inversion H5;subst.
-    apply n. apply sa_rcd...
-    { apply rt_type_drop with (E:=E)... }
-    { inversion w0... }
-    { simpl in H9.
-      rewrite <- !KeySetProperties.add_union_singleton in H9.
-      apply dom_add_subset in H9...
-      inversion H10;inversion H11... }
-    { inversion H10... }
-    { inversion H11... }
-    { intros. apply H12 with (i:=i).
-      + simpl. destruct (a == i)... subst i.
-        apply label_belong in H14.
-        inversion H11. exfalso...
-      + simpl. destruct (a == i)... subst i.
-        apply label_belong in H14.
-        inversion H11. exfalso...
-    }
-
-Qed.
-
-
-Lemma decidability : forall A B E,
-{sub E A B} + {~ sub E A B}.
-Proof with auto.
-  intros.
-  apply subtyping_dec with (k:=bindings_rec (mk_benv E) nil 0 A + 
-                               bindings_rec (mk_benv E) nil 0 B )...
-Qed.
