coq_fsub/coq_fsub_all/Rules.v
@@ -1,17 +1,18 @@
 Require Export Metalib.Metatheory.
 Require Export String.
 
+
 Inductive typ : Set :=
   | typ_nat : typ
+  | typ_top : typ
   | typ_bot : typ
   | typ_bvar : nat -> typ
   | typ_fvar : var -> typ
   | typ_arrow : typ -> typ -> typ
   | typ_all : typ -> typ -> typ
+  | typ_all_lb : typ -> typ -> typ
   | typ_mu : typ -> typ
-  | typ_label : var -> typ -> typ     
-  | typ_rcd_nil : typ
-  | typ_rcd_cons : var -> typ -> typ -> typ            
+  | typ_label : var -> typ -> typ              
 .
 
 Coercion typ_bvar : nat >-> typ.
@@ -23,13 +24,11 @@ Inductive exp : Set :=
   | exp_abs : typ -> exp -> exp
   | exp_app : exp -> exp -> exp
   | exp_tabs : typ -> exp -> exp
+  | exp_tabs_lb : typ -> exp -> exp
   | exp_tapp : exp -> typ -> exp
   | exp_nat : exp
   | exp_unfold : typ -> exp -> exp
   | exp_fold : typ -> exp -> exp
-  | exp_rcd_nil : exp
-  | exp_rcd_cons : var -> exp -> exp -> exp
-  | exp_rcd_proj : exp -> var -> exp
 .
 
 Coercion exp_bvar : nat >-> exp.
@@ -38,28 +37,23 @@ Coercion exp_fvar : atom >-> exp.
 Fixpoint open_tt_rec (K : nat) (U : typ) (T : typ) {struct T} : typ :=
   match T with
   | typ_nat         => typ_nat      
+  | typ_top         => typ_top
   | typ_bot         => typ_bot
   | typ_bvar J      => if K === J then U else (typ_bvar J)
   | typ_fvar X      => typ_fvar X 
   | typ_arrow T1 T2 => typ_arrow (open_tt_rec K U T1) (open_tt_rec K U T2)
   | typ_all T1 T2 => typ_all (open_tt_rec K U T1) (open_tt_rec (S K) U T2)
+  | typ_all_lb T1 T2 => typ_all_lb (open_tt_rec K U T1) (open_tt_rec (S K) U T2)
   | typ_mu T        => typ_mu (open_tt_rec (S K) U T)
-  | typ_label l T        => typ_label l (open_tt_rec K U T)
-  | typ_rcd_nil     => typ_rcd_nil
-  | typ_rcd_cons i T1 T2  => typ_rcd_cons i (open_tt_rec K U T1) (open_tt_rec K U T2)
+  | typ_label l T        => typ_label l (open_tt_rec K U T)                            
   end.
 
 
 Definition open_tt T U := open_tt_rec 0 U T.
 
-Inductive rt_type : typ -> Prop :=
-  | rt_type_rcd_nil :
-      rt_type typ_rcd_nil
-  | rt_type_rcd_cons : forall i T1 T2,
-      rt_type (typ_rcd_cons i T1 T2)
-.
-
 Inductive type : typ -> Prop :=
+  | type_top :
+      type typ_top
   | type_bot :
       type typ_bot
   | type_nat :
@@ -77,21 +71,20 @@ Inductive type : typ -> Prop :=
       type T1 ->
       (forall X, X `notin` L -> type (open_tt T2 (typ_fvar X))) ->
       type (typ_all T1 T2)
+  | type_all_lb : forall L T1 T2,
+      type T1 ->
+      (forall X, X `notin` L -> type (open_tt T2 (typ_fvar X))) ->
+      type (typ_all_lb T1 T2)
   | type_label: forall l A,
       type A ->
       type (typ_label l A)
-  | type_rcd_nil :
-      type typ_rcd_nil
-  | type_rcd_cons : forall i T1 T2,
-      type T1 ->
-      type T2 ->
-      rt_type T2 ->
-      type (typ_rcd_cons i T1 T2).
+.
 
 
 
 Fixpoint subst_tt (Z : atom) (U : typ) (T : typ) {struct T} : typ :=
   match T with
+  | typ_top => typ_top
   | typ_bot => typ_bot
   | typ_nat => typ_nat
   | typ_bvar J => typ_bvar J
@@ -100,55 +93,40 @@ Fixpoint subst_tt (Z : atom) (U : typ) (T : typ) {struct T} : typ :=
   | typ_mu T => typ_mu (subst_tt Z U T)
   | typ_label l T => typ_label l (subst_tt Z U T)                     
   | typ_all T1 T2 => typ_all (subst_tt Z U T1) (subst_tt Z U T2)
-  | typ_rcd_nil     => typ_rcd_nil
-  | typ_rcd_cons i T1 T2  => typ_rcd_cons i (subst_tt Z U T1) (subst_tt Z U T2)
+  | typ_all_lb T1 T2 => typ_all_lb (subst_tt Z U T1) (subst_tt Z U T2)
   end.
 
 Fixpoint fv_tt (T : typ) {struct T} : atoms :=
   match T with
+  | typ_top => {}
   | typ_bot => {}
   | typ_nat => {}
   | typ_bvar J => {}
   | typ_fvar X => {{ X }}
   | typ_arrow T1 T2 => (fv_tt T1) `union` (fv_tt T2)
-  | typ_all T1 T2 => (fv_tt T1) `union` (fv_tt T2)                                
+  | typ_all T1 T2 => (fv_tt T1) `union` (fv_tt T2)
+  | typ_all_lb T1 T2 => (fv_tt T1) `union` (fv_tt T2)
   | typ_mu T => (fv_tt T)
   | typ_label l T => (fv_tt T)
-  | typ_rcd_nil     => {}
-  | typ_rcd_cons i T1 T2  => fv_tt T1 \u fv_tt T2
   end.
 
 Inductive binding : Set :=
-| bind_sub : typ -> binding               
+| bind_sub : typ -> binding 
+| bind_sub_lb : typ -> binding 
 | bind_typ : typ -> binding.
 
 Definition env := list (atom * binding).
 Notation empty := (@nil (atom * binding)).
 
-Fixpoint Tlookup (i':var) (Tr:typ) : option typ :=
-  match Tr with
-  | (typ_rcd_cons i T1 T2) =>
-      if i == i' then Some T1 else Tlookup i' T2
-  | _ => None
-  end.
-
-Fixpoint collectLabel (T : typ) : atoms :=
-  match T with
-  | (typ_rcd_cons i T1 T2) => {{i}} \u collectLabel T2
-  | _ => {}
-  end.
-
-Fixpoint collectLabele (e: exp) : atoms :=
-  match e with
-  | (exp_rcd_cons i e1 e2) => {{i}} \u collectLabele e2
-  | _ => {}
-  end.
-
 Inductive WF : env -> typ -> Prop :=
+| WF_top : forall E, WF E typ_top
 | WF_bot : forall E, WF E typ_bot
 | WF_nat : forall E, WF E typ_nat
 | WF_var: forall U E (X : atom),
       binds X (bind_sub U) E ->
+      WF E (typ_fvar X)
+| WF_var_lb: forall U E (X : atom),
+      binds X (bind_sub_lb U) E ->
       WF E (typ_fvar X)
 | WF_arrow : forall E A B,
     WF E A ->
@@ -159,27 +137,25 @@ Inductive WF : env -> typ -> Prop :=
       (forall X : atom, X `notin` L ->
         WF (X ~ bind_sub T1 ++ E) (open_tt T2 X)) ->
       WF E (typ_all T1 T2)
+| WF_all_lb : forall L E T1 T2,
+      WF E T1 ->
+      (forall X : atom, X `notin` L ->
+        WF (X ~ bind_sub_lb T1 ++ E) (open_tt T2 X)) ->
+      WF E (typ_all_lb T1 T2)
 | WF_rec : forall L E A,
       (forall X, X \notin L -> 
-                 WF (X ~ bind_sub typ_bot ++ E) (open_tt A X)) ->
+                 WF (X ~ bind_sub typ_top ++ E) (open_tt A X)) ->
       (forall X, X \notin L -> 
-                 WF (X ~ bind_sub typ_bot ++ E) (open_tt A (typ_label X (open_tt A X)))) ->
+                 WF (X ~ bind_sub typ_top ++ E) (open_tt A (typ_label X (open_tt A X)))) ->
       WF E (typ_mu A)
 | WF_label: forall E A X,
     WF E A ->
     WF E (typ_label X A)
-| WF_rcd_nil : forall E,
-      WF E typ_rcd_nil
-| WF_rcd_cons : forall E i T1 T2,
-      WF E T1 ->
-      WF E T2 ->
-      rt_type T2 ->
-      i \notin (collectLabel T2) ->
-      WF E (typ_rcd_cons i T1 T2)
 .
 
 Fixpoint fl_tt (T : typ) {struct T} : atoms :=
   match T with
+  | typ_top => {}
   | typ_bot => {}
   | typ_nat => {}
   | typ_bvar J => {}
@@ -188,14 +164,14 @@ Fixpoint fl_tt (T : typ) {struct T} : atoms :=
   | typ_mu T => (fl_tt T)
   | typ_label X T => {{ X }} `union` fl_tt T
   | typ_all T1 T2 => (fl_tt T1) \u (fl_tt T2)
-  | typ_rcd_nil     => {}
-  | typ_rcd_cons i T1 T2  => {{i}} \u fl_tt T1 \u fl_tt T2
+  | typ_all_lb T1 T2 => (fl_tt T1) \u (fl_tt T2)
   end.
 
 Fixpoint fv_env (E:env) : atoms :=
   match E with
   | nil => {}
   | (x,bind_sub y)::E' => (fv_tt y) \u (fv_env E')
+  | (x,bind_sub_lb y)::E' => (fv_tt y) \u (fv_env E')
   | (x,bind_typ y)::E' => (fv_tt y) \u (fv_env E')
   end.
 
@@ -203,6 +179,7 @@ Fixpoint fl_env (E:env) : atoms :=
   match E with
   | nil => {}
   | (x,bind_sub y)::E' => (fl_tt y) \u (fl_env E')
+  | (x,bind_sub_lb y)::E' => (fl_tt y) \u (fl_env E')
   | (x,bind_typ y)::E' => (fl_tt y) \u (fl_env E')
   end.
 
@@ -214,6 +191,11 @@ Inductive wf_env : env -> Prop :=
       WF E T ->
       X `notin` dom E ->
       wf_env (X ~ bind_sub T ++ E)
+  | wf_env_subb : forall (E : env) (X : atom) (T : typ),
+      wf_env E ->
+      WF E T ->
+      X `notin` dom E ->
+      wf_env (X ~ bind_sub_lb T ++ E)
   | wf_env_typ : forall (E : env) (x : atom) (T : typ),
       wf_env E ->
       WF E T ->
@@ -228,12 +210,20 @@ Inductive sub : env -> typ -> typ -> Prop :=
     wf_env E ->
     WF E (typ_fvar X) ->
     sub E (typ_fvar X) (typ_fvar X)
+| sa_top : forall E A,
+    wf_env E ->
+    WF E A -> 
+    sub E A typ_top
 | sa_bot : forall E A,
     wf_env E ->
     WF E A -> 
     sub E typ_bot A
 | sa_trans_tvar : forall U E T X,
       binds X (bind_sub U) E ->
+      sub E U T ->
+      sub E (typ_fvar X) T
+| sa_trans_tvar_lb : forall U E T X,
+      binds X (bind_sub_lb U) E ->
       sub E T U ->
       sub E T (typ_fvar X)
 | sa_arrow: forall E A1 A2 B1 B2,
@@ -246,34 +236,33 @@ Inductive sub : env -> typ -> typ -> Prop :=
       (forall X : atom, X `notin` L ->
           sub (X ~ bind_sub S2 ++ E) (open_tt T1 X) (open_tt T2 X)) ->
       sub E (typ_all S1 T1) (typ_all S2 T2)
+| sa_all_lb : forall L E S1 S2 T1 T2,
+    sub E S1 S2 ->
+    sub E S2 S1 ->
+      (forall X : atom, X `notin` L ->
+          sub (X ~ bind_sub_lb S2 ++ E) (open_tt T1 X) (open_tt T2 X)) ->
+      sub E (typ_all_lb S1 T1) (typ_all_lb S2 T2)
 | sa_rec: forall L A1 A2 E,
     (forall X,
         X \notin L ->
-        WF (X ~ bind_sub typ_bot ++ E) (open_tt A1 X)) ->
+        WF (X ~ bind_sub typ_top ++ E) (open_tt A1 X)) ->
     (forall X,
         X \notin L ->
-        WF (X ~ bind_sub typ_bot ++ E) (open_tt A2 X)) ->
+        WF (X ~ bind_sub typ_top ++ E) (open_tt A2 X)) ->
     (forall X,
         X \notin L ->
-        sub (X ~ bind_sub typ_bot ++ E) (open_tt A1 (typ_label X (open_tt A1 X))) (open_tt A2 (typ_label X (open_tt A2 X)))) ->
+        sub (X ~ bind_sub typ_top ++ E) (open_tt A1 (typ_label X (open_tt A1 X))) (open_tt A2 (typ_label X (open_tt A2 X)))) ->
     sub E (typ_mu A1) (typ_mu A2)
 | sa_label: forall E X A B,
     sub E A B ->
     sub E (typ_label X A) (typ_label X B)
-| sa_rcd: forall A1 A2 E,
-    wf_env E ->
-    rt_type A1 ->
-    rt_type A2 ->
-    collectLabel A2 [<=] collectLabel A1 ->
-    WF E A1 -> WF E A2 ->
-    (forall i t1 t2, Tlookup i A1 = Some t1 ->  Tlookup i A2 = Some t2 -> sub E t1 t2) ->
-    sub E A1 A2
 .
 
 
 Definition subst_tb (Z : atom) (P : typ) (b : binding) : binding :=
   match b with
   | bind_sub T => bind_sub (subst_tt Z P T)
+  | bind_sub_lb T => bind_sub_lb (subst_tt Z P T)
   | bind_typ T => bind_typ (subst_tt Z P T)
   end.
 
@@ -285,12 +274,10 @@ Fixpoint open_te_rec (K : nat) (U : typ) (e : exp) {struct e} : exp :=
   | exp_abs V e1 => exp_abs  (open_tt_rec K U V)  (open_te_rec K U e1)
   | exp_app e1 e2 => exp_app  (open_te_rec K U e1) (open_te_rec K U e2)
   | exp_tabs V e1 => exp_tabs (open_tt_rec K U V)  (open_te_rec (S K) U e1)
+  | exp_tabs_lb V e1 => exp_tabs_lb (open_tt_rec K U V)  (open_te_rec (S K) U e1)
   | exp_tapp e1 V => exp_tapp (open_te_rec K U e1) (open_tt_rec K U V)
   | exp_unfold V e => exp_unfold (open_tt_rec K U V) (open_te_rec K U e)
   | exp_fold V e => exp_fold (open_tt_rec K U V) (open_te_rec K U e)
-  | exp_rcd_nil => exp_rcd_nil
-  | exp_rcd_cons i e1 e2 => exp_rcd_cons i (open_te_rec K U e1) (open_te_rec K U e2)
-  | exp_rcd_proj e1 i => exp_rcd_proj (open_te_rec K U e1) i     
   end.
 
 Fixpoint open_ee_rec (k : nat) (f : exp) (e : exp)  {struct e} : exp :=
@@ -301,23 +288,14 @@ Fixpoint open_ee_rec (k : nat) (f : exp) (e : exp)  {struct e} : exp :=
   | exp_abs V e1 => exp_abs V (open_ee_rec (S k) f e1)
   | exp_app e1 e2 => exp_app (open_ee_rec k f e1) (open_ee_rec k f e2)
   | exp_tabs V e1 => exp_tabs V (open_ee_rec k f e1)
+  | exp_tabs_lb V e1 => exp_tabs_lb V (open_ee_rec k f e1)
   | exp_tapp e1 V => exp_tapp (open_ee_rec k f e1) V
   | exp_unfold V e => exp_unfold V (open_ee_rec k f e)
-  | exp_fold V e => exp_fold V (open_ee_rec k f e)
-  | exp_rcd_nil => exp_rcd_nil
-  | exp_rcd_cons i e1 e2 => exp_rcd_cons i (open_ee_rec k f e1) (open_ee_rec k f e2)
-  | exp_rcd_proj e1 i => exp_rcd_proj (open_ee_rec k f e1) i   
+  | exp_fold V e => exp_fold V (open_ee_rec k f e)                            
   end.
 
 Definition open_te e U := open_te_rec 0 U e.
 Definition open_ee e1 e2 := open_ee_rec 0 e2 e1.
-
-Inductive rt_expr : exp -> Prop :=
-  | rt_expr_rcd_nil :
-      rt_expr exp_rcd_nil
-  | rt_expr_rcd_cons : forall i e1 e2,
-      rt_expr (exp_rcd_cons i e1 e2)
-.
 
 Inductive expr : exp -> Prop :=
   | expr_nat : expr exp_nat
@@ -335,6 +313,10 @@ Inductive expr : exp -> Prop :=
       type T ->
       (forall X : atom, X `notin` L -> expr (open_te e1 X)) ->
       expr (exp_tabs T e1)
+  | expr_tabs_lb : forall L T e1,
+      type T ->
+      (forall X : atom, X `notin` L -> expr (open_te e1 X)) ->
+      expr (exp_tabs_lb T e1)
   | expr_tapp : forall e1 V,
       expr e1 ->
       type V ->
@@ -347,29 +329,11 @@ Inductive expr : exp -> Prop :=
      type T ->
      expr e ->
      expr (exp_fold T e)
-  | expr_rcd_nil :
-     expr exp_rcd_nil
-  | expr_rcd_cons : forall i e1 e2,
-     expr e1 ->
-     expr e2 ->
-     rt_expr e2 ->
-     expr (exp_rcd_cons i e1 e2)
-  | expr_rcd_proj : forall i e,
-     expr e ->
-     expr (exp_rcd_proj e i)
 .
 
 Definition body_e (e : exp) :=
   exists L, forall x : atom, x `notin` L -> expr (open_ee e x).
 
-
-Fixpoint tlookup (i':var) (Er:exp) : option exp :=
-  match Er with
-  | (exp_rcd_cons i e1 e2) =>
-      if i == i' then Some e1 else tlookup i' e2
-  | _ => None
-  end.
-  
 
 Inductive typing : env -> exp -> typ -> Prop :=
   | typing_nat: forall G,
@@ -391,35 +355,29 @@ Inductive typing : env -> exp -> typ -> Prop :=
       (forall X : atom, X `notin` L ->
         typing (X ~ bind_sub V ++ E) (open_te e1 X) (open_tt T1 X)) ->
       typing E (exp_tabs V e1) (typ_all V T1)
+  | typing_tabs_lb : forall L E V e1 T1,
+      (forall X : atom, X `notin` L ->
+        typing (X ~ bind_sub_lb V ++ E) (open_te e1 X) (open_tt T1 X)) ->
+      typing E (exp_tabs_lb V e1) (typ_all_lb V T1)
   | typing_tapp : forall T1 E e1 T T2,
       typing E e1 (typ_all T1 T2) ->
+      sub E T T1 ->
+      typing E (exp_tapp e1 T) (open_tt T2 T)
+  | typing_tapp_lb : forall T1 E e1 T T2,
+      typing E e1 (typ_all_lb T1 T2) ->
       sub E T1 T ->
       typing E (exp_tapp e1 T) (open_tt T2 T)
   | typing_fold : forall G A T e ,
       sub G (typ_mu A) T ->
       typing G e (open_tt A T)  ->
       typing G (exp_fold T e) T
-  | typing_unfold : forall G A T e,
+ | typing_unfold : forall G A T e,
      typing G e A -> sub G A (typ_mu T) ->
      typing G (exp_unfold A e)  (open_tt T A)
   | typing_sub : forall S E e T,
       typing E e S ->
       sub E S T ->
       typing E e T
-  | typing_proj : forall G e T i Ti,
-      typing G e T ->
-      Tlookup i T = Some Ti ->
-      typing G (exp_rcd_proj e i) Ti
-  | typing_rcd_nil : forall G,
-      wf_env G ->
-      typing G exp_rcd_nil typ_rcd_nil
-  | typing_rcd_cons: forall G e1 e2 T1 T2 i,
-      typing G e1 T1 ->
-      typing G e2 T2 ->
-      rt_type T2 ->
-      rt_expr e2 ->
-      i \notin (collectLabele e2) ->
-      typing G (exp_rcd_cons i e1 e2) (typ_rcd_cons i T1 T2)
 .
 
 Inductive value : exp -> Prop :=
@@ -429,19 +387,15 @@ Inductive value : exp -> Prop :=
   | value_tabs : forall t1 T, 
       expr (exp_tabs T t1) ->
       value (exp_tabs T t1)
+  | value_tabs_lb : forall t1 T,
+      expr (exp_tabs_lb T t1) ->
+      value (exp_tabs_lb T t1)
   | value_nat:
       value exp_nat
   | value_fold: forall T e,
       type T ->
       value e ->
       value (exp_fold T e)
-  | value_rcd_nil:
-      value exp_rcd_nil
- | value_rcd_cons : forall i e1 e2,
-      value e1 ->
-      value e2 ->
-      rt_expr e2 ->
-      value (exp_rcd_cons i e1 e2)
 .
 
 Inductive step : exp -> exp -> Prop :=
@@ -465,6 +419,10 @@ Inductive step : exp -> exp -> Prop :=
       expr (exp_tabs T1 e1) ->
       type T2 ->
       step (exp_tapp (exp_tabs T1 e1) T2) (open_te e1 T2)
+ | step_tabs_lb : forall T1 e1 T2,
+    expr (exp_tabs_lb T1 e1) ->
+    type T2 ->
+    step (exp_tapp (exp_tabs_lb T1 e1) T2) (open_te e1 T2)
  | step_fld: forall S T v,
      value v ->
      type T ->
@@ -478,23 +436,9 @@ Inductive step : exp -> exp -> Prop :=
      step e e' ->
      type T ->
      step (exp_unfold T e) (exp_unfold T e')
- | step_projrcd: forall e i vi ,
-     value e ->
-     tlookup i e = Some vi->
-     step (exp_rcd_proj e i) vi
- | step_proj: forall e1 e2 i,
-     step e1 e2 ->
-     step (exp_rcd_proj e1 i) (exp_rcd_proj e2 i)
- | step_rcd_head: forall e1 e2 e i,
-     step e1 e2 ->
-     step (exp_rcd_cons i e1 e) (exp_rcd_cons i e2 e)
- | step_rcd_cons: forall v1 e1 e2 i,
-     value v1 ->
-     step e1 e2 ->
-     step (exp_rcd_cons i v1 e1) (exp_rcd_cons i v1 e2)
 .
 
-Hint Constructors rt_type rt_expr type WF wf_env sub expr typing step value: core.
+Hint Constructors type WF wf_env sub expr typing step value: core.
 
 
 Fixpoint fv_te (e : exp) {struct e} : atoms :=
@@ -505,12 +449,10 @@ Fixpoint fv_te (e : exp) {struct e} : atoms :=
   | exp_abs V e1  => (fv_tt V) `union` (fv_te e1)
   | exp_app e1 e2 => (fv_te e1) `union` (fv_te e2)
   | exp_tabs V e1 => (fv_tt V) `union` (fv_te e1)
+  | exp_tabs_lb V e1 => (fv_tt V) `union` (fv_te e1)
   | exp_tapp e1 V => (fv_tt V) `union` (fv_te e1)
   | exp_fold V e => fv_tt V \u fv_te e
   | exp_unfold V e => fv_tt V \u fv_te e
-  | exp_rcd_nil => {}
-  | exp_rcd_cons i e1 e2 => (fv_te e1) `union` (fv_te e2)
-  | exp_rcd_proj e1 i => (fv_te e1)
   end.
 
 Fixpoint fv_ee (e : exp) {struct e} : atoms :=
@@ -521,12 +463,10 @@ Fixpoint fv_ee (e : exp) {struct e} : atoms :=
   | exp_abs V e1 => (fv_ee e1)
   | exp_app e1 e2 => (fv_ee e1) `union` (fv_ee e2)
   | exp_tabs V e1 => (fv_ee e1)
+  | exp_tabs_lb V e1 => (fv_ee e1)
   | exp_tapp e1 V => (fv_ee e1)
   | exp_fold V e => fv_ee e
-  | exp_unfold V e => fv_ee e 
-  | exp_rcd_nil => {}
-  | exp_rcd_cons i e1 e2 => (fv_ee e1) `union` (fv_ee e2)
-  | exp_rcd_proj e1 i => (fv_ee e1)
+  | exp_unfold V e => fv_ee e                        
   end.
 
 Fixpoint subst_te (Z : atom) (U : typ) (e : exp) {struct e} : exp :=
@@ -537,12 +477,10 @@ Fixpoint subst_te (Z : atom) (U : typ) (e : exp) {struct e} : exp :=
   | exp_abs V e1 => exp_abs  (subst_tt Z U V)  (subst_te Z U e1)
   | exp_app e1 e2 => exp_app  (subst_te Z U e1) (subst_te Z U e2)
   | exp_tabs V e1 => exp_tabs (subst_tt Z U V)  (subst_te Z U e1)
+  | exp_tabs_lb V e1 => exp_tabs_lb (subst_tt Z U V)  (subst_te Z U e1)
   | exp_tapp e1 V => exp_tapp (subst_te Z U e1) (subst_tt Z U V)
   | exp_fold V e => exp_fold (subst_tt Z U V) (subst_te Z U e)
-  | exp_unfold V e => exp_unfold (subst_tt Z U V) (subst_te Z U e)
-  | exp_rcd_nil => exp_rcd_nil
-  | exp_rcd_cons i e1 e2 => exp_rcd_cons i (subst_te Z U e1) (subst_te Z U e2)
-  | exp_rcd_proj e1 i => exp_rcd_proj (subst_te Z U e1) i
+  | exp_unfold V e => exp_unfold (subst_tt Z U V) (subst_te Z U e)                           
   end.
 
 Fixpoint subst_ee (z : atom) (u : exp) (e : exp) {struct e} : exp :=
@@ -553,12 +491,10 @@ Fixpoint subst_ee (z : atom) (u : exp) (e : exp) {struct e} : exp :=
   | exp_abs V e1 => exp_abs V (subst_ee z u e1)
   | exp_app e1 e2 => exp_app (subst_ee z u e1) (subst_ee z u e2)
   | exp_tabs V e1 => exp_tabs V (subst_ee z u e1)
+  | exp_tabs_lb V e1 => exp_tabs_lb V (subst_ee z u e1)
   | exp_tapp e1 V => exp_tapp (subst_ee z u e1) V
   | exp_fold V e => exp_fold V (subst_ee z u e)
-  | exp_unfold V e => exp_unfold V (subst_ee z u e)
-  | exp_rcd_nil => exp_rcd_nil
-  | exp_rcd_cons i e1 e2 => exp_rcd_cons i (subst_ee z u e1) (subst_ee z u e2)
-  | exp_rcd_proj e1 i => exp_rcd_proj (subst_ee z u e1) i
+  | exp_unfold V e => exp_unfold V (subst_ee z u e)                                
   end.
 
 Inductive Mode := Pos | Neg. 
